src/Lib/DWT/VSTber_tlv_tag_serialize.v
@@ -2,72 +2,46 @@ Require Import Core.Core  Core.VstTactics Core.StructNormalizer VstLib DWT.Exec
         ErrorWithWriter.
 Require Import VST.floyd.proofauto.
 Require Import Clight.ber_tlv_tag ExecBer_tlv_tag_serialize.
-Require Import Core.Notations.
+Require Import Core.Notations Core.SepLemmas.
 
 Instance CompSpecs : compspecs. Proof. make_compspecs prog. Defined.
 Definition Vprog : varspecs. Proof. mk_varspecs prog. Defined.
 
 Open Scope IntScope.
 
-(* Fixpoint byte_length'_loop n z i l :=
-  match n with
-  | O => l
-  | S n => if z >> i == 0
-          then l 
-          else byte_length'_loop n z (i + Int.repr 7) (l + 1)
-  end.
-
-Definition byte_length' z := byte_length'_loop 4%nat z (Int.repr 7) 1.
-
-Definition serialize_tag' tval :=
-let fix serialize_tag' n i tval :=
-  match n with
-  | O => [tval & Int.repr 127]
-  | S n => (Int.repr 128 or (tval >> i & Int.repr 127)) 
-            :: serialize_tag' n (i - Int.repr 7) tval
-  end in 
- let s := byte_length' tval in 
- let n := Z.to_nat (Int.unsigned (s - 1)) in
- serialize_tag' n (s * Int.repr  7 - Int.repr 7) tval.
-
-Definition ber_tlv_tag_serialize' (tag size : int): list int * int :=
-  let tclass := tag & Int.repr 3 in 
-  let tval := tag >> Int.repr 2 in
-  if tval <=u Int.repr 30 then
-    if eq_dec size 0 
-    then ([], 1)
-    else ([(tclass << Int.repr 6) or tval], 1) 
-  else 
-    let required_size := byte_length' tval in
-    if eq_dec size 0 
-       then ([], required_size + 1)
-       else let buf0 := (tclass << Int.repr 6) or Int.repr 31 in
-            if (size - 1 <u required_size)
-            then ([buf0], required_size + 1)
-            else
-            (buf0 :: (serialize_tag' tag), required_size + 1). *)
-
 Definition ber_tlv_tag_serialize_spec' : ident * funspec :=
   DECLARE _ber_tlv_tag_serialize
-  WITH tag: int, bufp : val, size : int, buf_size : Z
+  WITH tag: int, buf_b : block, buf_ofs : ptrofs, size : int, buf_size : Z
   PRE[tuint, tptr tvoid, tuint]
     PROP((32 <= buf_size)%Z)
-    PARAMS(Vint tag; bufp; Vint size)
+    PARAMS(Vint tag; (Vptr buf_b buf_ofs); Vint size)
     GLOBALS()
     SEP(data_at Tsh (tarray tuchar buf_size)
-                     (default_val (tarray tuchar buf_size)) bufp )
+                    (default_val (tarray tuchar buf_size)) 
+                    (Vptr buf_b buf_ofs))
   POST[tuint]
     let (ls, z) := ber_tlv_tag_serialize' tag size in
     PROP()
     LOCAL(temp ret_temp (Vint z))
     SEP(if eq_dec ls [] 
         then data_at Tsh (tarray tuchar buf_size)
-                     (default_val (tarray tuchar buf_size)) bufp 
-         else data_at Tsh (tarray tuchar buf_size)
-                     (map (fun x => Vint (Int.zero_ext 8 x)) ls ++
-                          sublist (len ls) buf_size 
-                          (default_val (tarray tuchar buf_size)))
-                     bufp). 
+                         (default_val (tarray tuchar buf_size))
+                         (Vptr buf_b buf_ofs) 
+        else data_at Tsh (tarray tuchar buf_size)
+                         (map (fun x => Vint (Int.zero_ext 8 x)) ls ++
+                          sublist (len ls) buf_size (default_val (tarray tuchar buf_size)))
+                         (Vptr buf_b buf_ofs)).
+    (* SEP(if eq_dec ls [] 
+        then data_at Tsh (tarray tuchar buf_size)
+                     (default_val (tarray tuchar buf_size))
+                     (Vptr buf_b buf_ofs) 
+        else
+          data_at Tsh (tarray tuchar buf_size)
+                  (map (fun x => Vint (Int.zero_ext 8 x)) ls) 
+                  (Vptr buf_b buf_ofs) *
+          data_at Tsh (tarray tuchar (buf_size - len ls))
+                  (default_val (tarray tuchar (buf_size - len ls))) 
+                  (Vptr buf_b (buf_ofs + Ptrofs.repr (len ls))%ptrofs)).  *)
 
 Definition Gprog' := ltac:(with_library prog [ber_tlv_tag_serialize_spec']).
 
@@ -91,20 +65,23 @@ Proof.
     break_if;
     autorewrite with norm in *; try nia.
     auto.  }
-  - forward_if (
+  - remember (Int.zero_ext 8 (Int.or (Int.shl ((tag & Int.repr 3)) (Int.repr 6)) 
+                                (tag >> Int.repr 2)%int)) as e0.
+    forward_if (
        PROP()
        LOCAL()
        SEP(if eq_dec size 0 
-           then data_at_ Tsh (tarray tuchar buf_size) bufp 
-           else (data_at Tsh (tarray tuchar buf_size)
-    (upd_Znth 0 (default_val (tarray tuchar buf_size))
-       (Vint
-          (Int.zero_ext 8
-             (Int.or (Int.shl 
-                        ((tag & Int.repr 3)) (Int.repr 6)) 
-                     (tag >> Int.repr 2)%int)))) bufp))).
+           then data_at_ Tsh (tarray tuchar buf_size) (Vptr buf_b buf_ofs) 
+           else data_at Tsh (tarray tuchar buf_size)
+                        (upd_Znth 0 (default_val (tarray tuchar buf_size))
+                                  (Vint e0)) (Vptr buf_b buf_ofs))).
+        (* (data_at Tsh (tarray tuchar buf_size) [Vint e0] (Vptr buf_b buf_ofs) *
+          data_at Tsh (tarray tuchar (buf_size - 1))
+                  (default_val (tarray tuchar (buf_size - 1))) 
+                  (Vptr buf_b (buf_ofs + 1)%ptrofs)))). *)
     + forward. 
-      rewrite_if_b. entailer!.
+      rewrite_if_b.
+      entailer!.
     + forward.
       rewrite_if_b.
       entailer!.
@@ -124,6 +101,7 @@ Proof.
         entailer!.
         nia.
   - (* 30 < tag *)
+    remember (Int.zero_ext 8 (((tag & Int.repr 3) << Int.repr 6) or Int.repr 31)) as e0. 
     assert (((tag >> Int.repr 2) <=u Int.repr 30) = false) as C.
     { unfold Int.ltu.
       break_if;
@@ -132,43 +110,51 @@ Proof.
     forward_if (
        PROP()
        LOCAL(if eq_dec size 0 
-             then temp _buf__1 bufp
-             else temp _buf__1 (offset_val 1 bufp)  ;
+             then temp _buf__1 (Vptr buf_b buf_ofs)
+             else temp _buf__1 (offset_val 1 (Vptr buf_b buf_ofs))  ;
              if eq_dec size 0 
              then temp _size (Vint size)
              else temp _size (Vint (size - 1));
-            temp _tval (Vint (tag >> Int.repr 2)))
+            temp _tval (Vint tval))
        SEP(if eq_dec size 0 
            then data_at Tsh (tarray tuchar buf_size)
-                     (default_val (tarray tuchar buf_size)) bufp  
-           else (data_at Tsh (tarray tuchar buf_size)
-    (upd_Znth 0 (default_val (tarray tuchar buf_size))
-       (Vint
-          (Int.zero_ext 8
-             (Int.or (Int.shl 
-                        ((tag & Int.repr 3)) (Int.repr 6)) 
-                     (Int.repr 31))))) bufp))).
-    + unfold tarray. 
-      erewrite split2_data_at_Tarray_tuchar with (n1 := 1%Z). 
+                     (default_val (tarray tuchar buf_size)) (Vptr buf_b buf_ofs)  
+           else data_at Tsh (tarray tuchar buf_size)
+                        (upd_Znth 0 (default_val (tarray tuchar buf_size))
+                                  (Vint e0)) (Vptr buf_b buf_ofs))).
+    + remember (default_val (tarray tuchar buf_size)) as default_list.
+      rewrite <- LB.
+      erewrite split_data_at_sublist_tuchar with (j := 1%Z).
       erewrite sublist_one.
       erewrite data_at_tuchar_singleton_array_eq.
       Intros.
       repeat forward.
       repeat rewrite_if_b.
       entailer!.
-      erewrite <- data_at_tuchar_singleton_array_eq.
       erewrite upd_Znth_unfold.
       erewrite sublist_nil.
       erewrite app_nil_l.
-      erewrite split2_data_at_Tarray_app with (mid := 1%Z).
-      replace (len (default_val (tarray tuchar buf_size))) with buf_size
-        by eassumption. (* rewrite cannot find the term - bug? *)
+      assert (forall (cs : compspecs) i ls' ls sh b ofs z,
+      ls = i::ls'  -> 
+      z = Zlength ls' ->
+      (Ptrofs.unsigned ofs + Zlength ls < Ptrofs.modulus)%Z -> 
+      data_at sh (tarray tuchar (Zlength ls)) ls (Vptr b ofs) =
+      (data_at sh tuchar i (Vptr b ofs) *
+      data_at sh (tarray tuchar z) ls'
+              (Vptr b (Ptrofs.add ofs Ptrofs.one))))%logic as SP by admit.
+       remember (default_val (tarray tuchar buf_size)) as default_list.
+       remember (Int.zero_ext 8 (((tag & Int.repr 3) << Int.repr 6) or Int.repr 31)) as e0.
+      erewrite <- SP  with (ls :=  ([Vint e0] ++ sublist 1 (len default_list) default_list)).
+      replace  buf_size with (len ([Vint e0] ++ sublist 1 (len default_list) default_list)).
       entailer!.
+      admit.
+      admit.
       all: try nia;
         unfold default_val;
         simpl;
         try erewrite Zlength_list_repeat;
         try nia; auto.
+      all: admit.
     + forward.
       repeat rewrite_if_b.
       entailer!.
@@ -182,9 +168,9 @@ Proof.
                  temp _i (Vint i);
                  temp _required_size (Vint j);
                  temp _size (Vint size);
-                 temp _buf__1 bufp)
+                 temp _buf__1 (Vptr buf_b buf_ofs))
           SEP (data_at Tsh (tarray tuchar buf_size)
-                       (default_val (tarray tuchar buf_size)) bufp))
+                       (default_val (tarray tuchar buf_size)) (Vptr buf_b buf_ofs)))
       break: (EX i: int, 
                  PROP (((tag >> Int.repr 2) >> i == 0)%int = true 
                        \/ Int.unsigned i >= 8 * sizeof tuint)
@@ -192,9 +178,9 @@ Proof.
                        temp _tval (Vint (tag >> Int.repr 2));
                        temp _i (Vint i);
                        temp _size (Vint size);
-                       temp _buf__1 bufp)
+                       temp _buf__1 (Vptr buf_b buf_ofs))
                  SEP (data_at Tsh (tarray tuchar buf_size)
-                              (default_val (tarray tuchar buf_size)) bufp)).
+                              (default_val (tarray tuchar buf_size)) (Vptr buf_b buf_ofs))).
          * (* Pre implies Inv *)
            Exists (Int.repr 7).
            Exists 1.
@@ -230,6 +216,7 @@ Proof.
            replace (Int.unsigned 0) with 0%Z in * by auto with ints. 
            assert (1 <= Int.unsigned (byte_length' tval))%Z as BL.
            { unfold byte_length'.
+             unfold byte_length'_loop.
              repeat break_if; discriminate. }
            nia.
      ++ repeat forward.        
@@ -240,14 +227,14 @@ Proof.
                  temp _i (Vint i);
                  temp _required_size (Vint j);
                  temp _size (Vint (size - 1));
-                 temp _buf__1  (offset_val 1 bufp))
+                 temp _buf__1  (offset_val 1 (Vptr buf_b buf_ofs)))
            SEP ((data_at Tsh (tarray tuchar buf_size)
     (upd_Znth 0 (default_val (tarray tuchar buf_size))
        (Vint
           (Int.zero_ext 8
              (Int.or (Int.shl 
                         ((tag & Int.repr 3)) (Int.repr 6)) 
-                     (Int.repr 31))))) bufp)))
+                     (Int.repr 31))))) (Vptr buf_b buf_ofs))))
       break: (EX i: int, 
                  PROP (((tag >> Int.repr 2) >> i == 0)%int = true 
                        \/ Int.unsigned i >= 8 * sizeof tuint)
@@ -255,14 +242,14 @@ Proof.
                        temp _tval (Vint (tag >> Int.repr 2));
                        temp _i (Vint i);
                        temp _size (Vint (size - 1));
-                       temp _buf__1  (offset_val 1 bufp))
+                       temp _buf__1  (offset_val 1 (Vptr buf_b buf_ofs)))
                   SEP ((data_at Tsh (tarray tuchar buf_size)
     (upd_Znth 0 (default_val (tarray tuchar buf_size))
        (Vint
           (Int.zero_ext 8
              (Int.or (Int.shl 
                         ((tag & Int.repr 3)) (Int.repr 6)) 
-                     (Int.repr 31))))) bufp))).
+                     (Int.repr 31))))) (Vptr buf_b buf_ofs)))).
          * (* Pre implies Inv *)
            Exists (Int.repr 7).
            Exists 1.
@@ -307,66 +294,53 @@ Proof.
            entailer!.
            nia.
            forward.
-           entailer!.
-           admit. (* do we assume that buf + 1 is not null? *)
            forward.
            remember (default_val (tarray tuchar buf_size)) as default_list.
-           remember (Int.zero_ext 8 (((tag & Int.repr 3) << Int.repr 6) or Int.repr 31)) as e0.
-(*
-           Fixpoint serialize_tag_loop  n i tval :=
-             match n with
-             | O => []
-             | S n => (Int.repr 128 or (tval >> i & Int.repr 127)) 
-                       :: serialize_tag_loop n (i - Int.repr 7) tval
-             end. 
-           Definition serialize_tag tval :=
-             let s := byte_length' tval in 
-             let n := Z.to_nat (Int.unsigned (s - 1)) in
-             serialize_tag_loop n (s * Int.repr  7 - Int.repr 7) tval. *)
-
-(* [Vint (Int.repr 128 or ((tval >> (i - Int.repr (v*7))) & (Int.repr 127)))] *)
-           forward_loop  (EX i : int, EX v : Z, EX ls : list val, 
-                             PROP ()
-                             LOCAL ( temp _tval (Vint (tag >> Int.repr 2));
-                                     temp _i (Vint i);
-                                     temp _required_size (Vint (byte_length' tval));
-                                     temp _size (Vint (size - 1));
-                                     temp _buf__1 (offset_val (v + 1) bufp);
-                                     temp _end
-       (force_val (sem_binary_operation' Osub (tptr tuchar) tint
-             (eval_binop Oadd (tptr tuchar) tuint (offset_val 1 bufp) 
-                         (Vint (byte_length' tval))) (Vint (Int.repr 1)))))
-          SEP (data_at Tsh (tarray tuchar 1) [Vint e0] bufp;
-               data_at Tsh (tarray tuchar v) (ls)
-                        (offset_val 1 bufp);
-                        data_at Tsh (tarray tuchar (buf_size - v)) 
-                        (skipn (Z.to_nat v) default_list) (offset_val (v + 1) bufp)))
-          break:(EX i: Z, PROP ()
-                          LOCAL ( temp _tval (Vint (tag >> Int.repr 2));
-                                  temp _i (Vint (Int.repr i));
+           forward_loop (
+               EX i : int, EX v : Z, EX ls : list int, 
+                           PROP ()
+                           LOCAL (temp _tval (Vint (tag >> Int.repr 2));
+                                  temp _i (Vint i);
                                   temp _required_size (Vint (byte_length' tval));
-                                  temp _size (Vint size);
-                                  temp _buf__1 (offset_val i bufp))
-                          SEP (data_at Tsh (tarray tuchar buf_size)
-                       (default_val (tarray tuchar buf_size)) (offset_val i bufp))).
+                                  temp _size (Vint (size - 1));
+                                  temp _buf__1 (offset_val (v + 1) (Vptr buf_b buf_ofs));
+                                  temp _end
+          (force_val (sem_binary_operation' Osub (tptr tuchar) tint
+             (eval_binop Oadd (tptr tuchar) tuint (offset_val 1 (Vptr buf_b buf_ofs)) 
+                         (Vint (byte_length' tval))) (Vint (Int.repr 1)))))
+          SEP (data_at Tsh (tarray tuchar 1) [Vint e0] (Vptr buf_b buf_ofs);
+               data_at Tsh (tarray tuchar v) (map Vint ls)
+                        (offset_val 1 (Vptr buf_b buf_ofs));
+               data_at Tsh (tarray tuchar (buf_size - v)) 
+                        (skipn (Z.to_nat v) default_list) 
+                        (offset_val (v + 1) (Vptr buf_b buf_ofs))))
+
+          break: (EX i: int, EX ls : list int,
+
+                       PROP (let s := byte_length' tag in 
+                             let n := Z.to_nat (Int.unsigned (s - 1)) in
+                             ls = serialize_tag_loop n
+                                (s * Int.repr  7 - Int.repr 7)%int tag)
+
+                       LOCAL (temp _tval (Vint (tag >> Int.repr 2));
+                              temp _i (Vint i);
+                              temp _required_size (Vint (byte_length' tval));
+                              temp _size (Vint (size - 1));
+                              temp _buf__1 (offset_val (len ls + 1) (Vptr buf_b buf_ofs)))
+
+                       SEP (data_at Tsh (tarray tuchar 1) [Vint e0] (Vptr buf_b buf_ofs);
+                            data_at Tsh (tarray tuchar (len ls)) (map Vint ls)
+                                    (offset_val 1 (Vptr buf_b buf_ofs));
+                            data_at Tsh (tarray tuchar (buf_size - (Zlength ls))) 
+                                    (sublist (len ls) buf_size default_list) 
+                                    (offset_val ((Zlength ls) + 1) (Vptr buf_b buf_ofs)))).
           *** Exists (i - Int.repr 7).
               Exists 0%Z.
-              Exists (@nil val).
+              Exists (@nil int).
               entailer!.
               erewrite data_at_tuchar_zero_array_eq.
               entailer!.
               all: admit.
-              (* Search upd_Znth.
-              erewrite upd_Znth_unfold.
-              erewrite sublist_nil.
-              erewrite app_nil_l.
-              assert (forall (a : val) ls, a :: ls = [a] ++ ls) as LS.
-              { intros.
-                destruct ls; econstructor. }
-              erewrite <- LS.
-              simpl.
-              admit.
-              admit. *)
           *** Intros j v ls.
               forward_if.
               admit.
@@ -379,28 +353,198 @@ Proof.
               forward.
               entailer!.
               admit.
-              repeat forward.
-              
+              repeat forward.              
               Exists (j - Int.repr 7).
               Exists (v + 1)%Z.
-              Exists (ls ++ [Vint (Int.repr 128 or ((tval >> j) & (Int.repr 127)))]).
+              Exists (ls ++ [Int.repr 128 or ((tval >> j) & (Int.repr 127))]).
               entailer!.
               all: try nia.
               1-4: admit.
               forward.
-          *** Intro x.
+              Exists j.
+              Exists ls.
+              entailer!.
+              assert (len ls = v) by admit.              
+              subst.
+              admit.
+               assert (len ls = v) by admit.              
+              subst.
+              entailer!.
+              admit.
+          *** Intros i0 ls.
               unfold tarray. 
-              erewrite split2_data_at_Tarray_tuchar with (n1 := 1%Z). 
-              Intros.
+              erewrite split2_data_at_Tarray_tuchar with (n0 := (buf_size - (len ls))%Z) 
+                                                         (n1 := 1%Z).
               erewrite sublist_one.
-              erewrite data_at_tuchar_singleton_array_eq.
+              erewrite data_at_tuchar_singleton_array_eq at 1.
+              erewrite data_at_tuchar_singleton_array_eq at 1.
+              Intros.
               forward.
+              erewrite <- data_at_tuchar_singleton_array_eq at 1.
+              erewrite <- data_at_tuchar_singleton_array_eq at 1.
+              assert ((field_address0 (Tarray tuchar (buf_size - len ls) noattr) (SUB 1)
+          (offset_val (len ls + 1) (Vptr buf_b buf_ofs))) = offset_val 1 (offset_val (len ls + 1) (Vptr buf_b buf_ofs))).
+              { 
+                rewrite field_address0_offset.
+                simpl.
+                reflexivity.
+                econstructor.
+                easy.
+                repeat split.
+                simpl; autorewrite with norm.
+                admit.
+                                constructor.
+                intros.
+                repeat econstructor.
+                simpl; autorewrite with norm.
+                reflexivity.
+                all: try nia || auto with zarith.
+                autorewrite with sublist.
+                simpl.
+                admit.
+              }
+              rewrite H4.
               unfold POSTCONDITION.
               unfold abbreviate. 
               break_let.
               forward.
                unfold ber_tlv_tag_serialize' in *; rewrite C in *;
               rewrite_if_b.
+               rewrite H2 in *.
+               inversion Heqp.
+                rewrite_if_b.
+                rewrite if_false by congruence.
+               
+               all: try nia.
+               remember ((((tag & Int.repr 3) << Int.repr 6) or Int.repr 31)) as e0.   
+               unfold serialize_tag'.
+               rewrite <- H3.
+               clear H3.
                entailer!.
+               remember (default_val (tarray tuchar buf_size)) as default_list.
+               remember (Int.zero_ext 8 (((tag & Int.repr 3) << Int.repr 6) or Int.repr 31)) as e0.
+               remember (Int.zero_ext 8 ((tag >> Int.repr 2) & Int.repr 127)) as e_n.
+               unfold offset_val.
+               simpl.
+ assert (forall (cs : compspecs) sh ls1 ls2 b ofs j1 j2,
+    Zlength ls1 = j1 ->
+    Zlength ls2 = j2 ->
+    data_at sh (tarray tuchar (j1 + j2)) (ls1 ++ ls2) (Vptr b ofs) =
+    (data_at sh (tarray tuchar j1) ls1 (Vptr b ofs) *
+     data_at sh (tarray tuchar j2) ls2
+             (Vptr b (Ptrofs.add ofs (Ptrofs.repr j1))))%logic) as SP by admit.
+ unfold tarray in *.
+               erewrite <- SP.
+               replace (1 + len ls)%Z with (len ls + 1)%Z by nia.
+               erewrite <- SP.
+                erewrite <- SP.
+                normalize.
+                autorewrite with norm.
+             (*  replace (Vint e_n) with (Znth 0 (Vint e_n :: skipn (length ls - 1)%nat default_list)).
+               erewrite <- sublist_one with (hi := 1%Z).
+            
+               replace (skipn (Datatypes.length ls) default_list) with 
+                 (Vint e_n :: skipn (length ls - 1)%nat default_list) at 1.  
+               replace (buf_size - len ls - 1)%Z with ((buf_size - len ls) - 1)%Z by nia.
+               rewrite sepcon_assoc.
+               unfold tarray.
+               erewrite <- split2_data_at_Tarray_tuchar.
+               replace (len ((((tag & Int.repr 3) << Int.repr 6) or Int.repr 31) :: ls)) with
+                   (len ls + 1)%Z.
+               replace (map (fun x : int => Vint (Int.zero_ext 8 x)) ls) with (map Vint ls).
+               replace (Vint e0 :: map Vint ls) with ([Vint e0] ++ (map Vint ls)).
+               unfold offset_val.
+               break_match.
                admit.
+               admit.
+               admit.
+               admit.
+               admit.
+               pose proof combine_data_at_sublist_tuchar.
+               unfold tarray in *.
+               replace (data_at Tsh (Tarray tuchar buf_size noattr)
+        (([Vint e0]
+           ++ map Vint ls) 
+           ++ sublist (len ls + 1) buf_size default_list) 
+        (Vptr b i1))
+              with
+                (data_at Tsh (Tarray tuchar
+                (len (([Vint e0] ++ map Vint ls) 
+                        ++ sublist (len ls + 1) buf_size default_list))
+                noattr)
+                         (([Vint e0] ++ 
+                                     map Vint ls)
+                            ++ sublist (len ls + 1) buf_size default_list) 
+                         (Vptr b i1)).
+                erewrite H16 with (j := 1%Z).
+                replace (len (([Vint e0] ++ map Vint ls) ++ sublist (len ls + 1) buf_size default_list) - 1)%Z
+               with (len ((map Vint ls) ++ sublist (len ls + 1) buf_size default_list)).
+                instantiate (2 := [Vint e0]).
+                 instantiate (1 :=  (map Vint ls) ++ sublist (len ls + 1) buf_size default_list).
+                 replace  (data_at Tsh
+         (Tarray tuchar
+            (len (([Vint e0] ++ map Vint ls) ++ sublist (len ls + 1) buf_size default_list) - 1)
+            noattr) (map Vint ls ++ sublist (len ls + 1) buf_size default_list)
+         (Vptr b (i1 + Ptrofs.repr 1)%ptrofs))%logic
+                          with 
+
+ (data_at Tsh
+         (Tarray tuchar
+            (len ((map Vint ls) ++ sublist (len ls + 1) buf_size default_list))
+            noattr) (map Vint ls ++ sublist (len ls + 1) buf_size default_list)
+         (Vptr b (i1 + Ptrofs.repr 1)%ptrofs))%logic.
+                  erewrite H16 with (j := len ls) (ls1 :=  (map Vint ls))
+                                    (ls2 := (Vint e_n :: skipn (Datatypes.length ls - 1) default_list)).
+                  entailer!.
+
+
+                 replace  (data_at Tsh
+         (Tarray tuchar
+            (len (([Vint e0] ++ map Vint ls) ++ sublist (len ls + 1) buf_size default_list) - 1)
+            noattr) [Vint e0] (Vptr b (i1 + Ptrofs.repr 1))) with
+( data_at Tsh
+         (Tarray tuchar
+            (len (map Vint ls) ++ sublist (len ls + 1) buf_size default_list))
+            noattr) [Vint e0] (Vptr b (i1 + Ptrofs.repr 1)).
+               autorewrite with sublist.
+                erewrite H16.
+ (ls := [Vint e0]).
+                
+                
+
+               replace buf_size with
+                   (len (([Vint e0] ++ map Vint ls) ++ sublist (len ls + 1) buf_size default_list))
+                   at 2.
+               erewrite H16.
+               replace (len ls) with (len (Vint e0:: map Vint ls) - 1)%Z.
+               erewrite <- H16.
+                erewrite <- H16.
+               replace (len ls) with (len (e0::ls) - 1)%Z.
+               replace  (data_at Tsh (Tarray tuchar 1 noattr) [Vint e0] (Vptr b i1) *
+   data_at Tsh (Tarray tuchar (len (e0 :: ls) - 1) noattr) (map Vint ls)
+     (Vptr b (i1 + Ptrofs.repr 1)%ptrofs))%logic with
+                    (data_at Tsh (Tarray tuchar (len (e0 :: ls)) noattr) (Vint e0:: (map Vint ls)) (Vptr b i1)). admit.
+               erewrite H16.
+
+               replace buf_size with
+                   (len (([Vint e0] ++ map Vint ls) ++ sublist (len ls + 1) buf_size default_list))
+                   at 2.
+               erewrite H16.
+               
+
+               assert (forall (cs : compspecs) sh ls ls1 ls2 b ofs j,
+                           (Ptrofs.unsigned ofs + Zlength ls < Ptrofs.modulus)%Z ->
+                           0 <= j <= Zlength ls ->
+                           ls = ls1 ++ ls2 ->
+                           data_at sh (tarray tuchar (Zlength ls)) ls (Vptr b ofs) =
+                           (data_at sh (tarray tuchar j) ls1 (Vptr b ofs) *
+                            data_at sh (tarray tuchar (Zlength ls - j)) ls2
+                                    (Vptr b (ofs + (Ptrofs.repr j))%ptrofs)))%logic.
+               { intros.
+                  erewrite  split_data_at_sublist_tuchar.
+               
+               erewrite <- split_data_at_sublist_tuchar.
+               Search data_at sublist.
+               
+               all: admit. *)
 Admitted.
